Splinter/Betree/PivotBetreeRefinement.i.dfy
@@ -5,4 +5,297 @@ include "PivotBetree.i.dfy"
 
 module PivotBetreeRefinement
 {
+  import opened Options
+  import opened KeyType
+  import opened StampedMapMod
+  import TotalKMMapMod
+  import opened ValueMessage
+  import opened MsgHistoryMod
+  import opened LSNMod
+  import opened Sequences
+  import opened Buffers
+  import opened MemtableMod
+  import opened Upperbounded_Lexicographic_Byte_Order_Impl
+  import opened Upperbounded_Lexicographic_Byte_Order_Impl.Ord
+  import opened BoundedPivotsLib
+  import opened PivotBetree
+  import PagedBetree
+
+  function INode(node: BetreeNode) : PagedBetree.BetreeNode
+    requires node.WF()
+  {
+    if node.Nil?
+    then PagedBetree.Nil
+    else PagedBetree.BetreeNode(
+      node.buffers,
+      PagedBetree.ChildMap(imap key | AnyKey(key) ::
+        assert WFChildren(node.children); // trigger
+        if key in node.KeySet() then INode(node.Child(key)) else PagedBetree.Nil))
+  }
+
+  function IStampedBetree(stampedBetree: StampedBetree) : PagedBetree.StampedBetree
+    requires stampedBetree.WF()
+  {
+    PagedBetree.StampedBetree(INode(stampedBetree.root), stampedBetree.seqEnd)
+  }
+
+  function ILbl(lbl: TransitionLabel) : PagedBetree.TransitionLabel
+  {
+    match lbl
+      case QueryLabel(endLsn, key, value) => PagedBetree.QueryLabel(endLsn, key, value)
+      case PutLabel(puts) => PagedBetree.PutLabel(puts)
+      case QueryEndLsnLabel(endLsn) => PagedBetree.QueryEndLsnLabel(endLsn)
+      case FreezeAsLabel(stampedBetree) =>PagedBetree.FreezeAsLabel(
+        if stampedBetree.WF()
+        then IStampedBetree(stampedBetree)
+        else PagedBetree.EmptyStampedBetree())
+      case InternalLabel() => PagedBetree.InternalLabel()
+  }
+
+  function I(v: Variables) : PagedBetree.Variables
+    requires v.WF()
+  {
+    PagedBetree.Variables(v.memtable, IStampedBetree(v.stampedBetree))
+  }
+
+  predicate Inv(v: Variables)
+  {
+    && v.WF()
+  }
+
+  lemma INodeWF(node: BetreeNode)
+    requires node.WF()
+    ensures INode(node).WF()
+  {
+    if node.BetreeNode? {
+      forall k | AnyKey(k) ensures INode(node).children.mapp[k].WF() {
+        if k in node.KeySet() {
+          INodeWF(node.Child(k));
+        }
+      }
+    }
+  }
+
+  lemma InvNext(v: Variables, v': Variables, lbl: TransitionLabel)
+    requires Inv(v)
+    requires Next(v, v', lbl)
+    ensures Inv(v')
+  {
+    assume false;
+  }
+
+  function IPath(path: Path) : PagedBetree.Path
+    requires path.Valid()
+  {
+    PagedBetree.Path(INode(path.node), path.key, path.Target().KeySet(), 0)
+  }
+
+  lemma ValidPathRefines(path: Path)
+    requires path.Valid()
+    ensures IPath(path).Valid()
+  {
+    assume false;
+  }
+
+  lemma PathTargetRefines(path: Path)
+    requires path.Valid()
+    ensures INode(path.Target()) == IPath(path).Target()
+  {
+    assume false;
+  }
+
+  function IReceiptLine(line: QueryReceiptLine) : PagedBetree.QueryReceiptLine
+    requires line.WF()
+  {
+    PagedBetree.QueryReceiptLine(INode(line.node), line.result)
+  }
+
+  function IReceipt(receipt: QueryReceipt) : PagedBetree.QueryReceipt
+    requires receipt.Valid()
+  {
+    PagedBetree.QueryReceipt(receipt.key, INode(receipt.root),
+      seq(|receipt.lines|, i requires 0<=i<|receipt.lines| => IReceiptLine(receipt.lines[i])))
+  }
+
+  function SplitChildKeys(step: Step) : iset<Key>
+    requires step.InternalSplitStep?
+  {
+    step.path.Target().ChildDomain(step.childIdx).KeySet()
+  }
+
+  // Hide iset quantifier mentioning lt, which is a trigger party
+  function {:opaque} SplitLeftKeys(step: Step) : iset<Key>
+    requires step.InternalSplitStep?
+  {
+//    iset key | key in SplitChildKeys(step) && lt(Element(key), Element(step.splitKey)) XXX
+    iset key | true
+  }
+
+  function IStep(v: Variables, v': Variables, lbl: TransitionLabel, step: Step) : PagedBetree.Step
+    requires NextStep(v, v', lbl, step) // Fancy (lazy) way of assuming all the step parts are WF
+  {
+    match step {
+      case QueryStep(receipt) => PagedBetree.QueryStep(IReceipt(receipt))
+      case PutStep() => PagedBetree.PutStep()
+      case QueryEndLsnStep() => PagedBetree.QueryEndLsnStep()
+      case FreezeAsStep() => PagedBetree.FreezeAsStep()
+      case InternalGrowStep() => PagedBetree.InternalGrowStep()
+      case InternalSplitStep(path, childIdx, splitKey) => 
+        if !path.Valid()
+        then PagedBetree.InternalSplitStep(
+          PagedBetree.Path(PagedBetree.Nil, path.key, iset{}, 0), iset{}, iset{})
+        else
+          var rightKeys := SplitChildKeys(step) - SplitLeftKeys(step);
+          PagedBetree.InternalSplitStep(IPath(path), SplitLeftKeys(step), rightKeys)
+      case InternalFlushStep(path, childIdx) => 
+        PagedBetree.InternalFlushStep(IPath(path), path.Target().ChildDomain(childIdx).KeySet())
+      case InternalCompactStep(path, compactedNode) => 
+        PagedBetree.InternalCompactStep(IPath(path), INode(compactedNode))
+    }
+  }
+
+  lemma InitRefines(v: Variables, stampedBetree: StampedBetree)
+    requires Init(v, stampedBetree)
+    ensures PagedBetree.Init(I(v), IStampedBetree(stampedBetree))
+  {
+    INodeWF(stampedBetree.root);
+  }
+
+  lemma ValidReceiptRefines(receipt: QueryReceipt)
+    requires receipt.Valid()
+    ensures IReceipt(receipt).Valid()
+  {
+    var ir := IReceipt(receipt);
+    forall i:nat | i < |ir.lines| ensures ir.lines[i].WF() {
+      INodeWF(receipt.lines[i].node);
+    }
+    forall i:nat | i < |ir.lines| - 1 ensures ir.ChildLinkedAt(i) {
+      assert receipt.ChildLinkedAt(i);
+    }
+    forall i:nat | i < |ir.lines| - 1 ensures ir.ResultLinkedAt(i) {
+      assert receipt.ResultLinkedAt(i);
+    }
+  }
+
+  lemma AllKeysInTotalDomain(key: Key)
+    ensures key in TotalDomain().KeySet()
+    ensures TotalDomain().Contains(key)
+  {
+    SmallestElementLte(Element(key));
+    assert TotalDomain().Contains(key) by { TotalDomain().reveal_Contains(); }
+  }
+
+  lemma InternalGrowStepRefines(v: Variables, v': Variables, lbl: TransitionLabel, step: Step)
+    requires Inv(v)
+    requires NextStep(v, v', lbl, step)
+    requires step.InternalGrowStep?
+    ensures v'.WF()
+    ensures PagedBetree.NextStep(I(v), I(v'), ILbl(lbl), IStep(v, v', lbl, step))
+  {
+    INodeWF(v.stampedBetree.root);
+    INodeWF(v'.stampedBetree.root);
+
+    assert I(v').stampedBetree.root.children.mapp.Keys == AllKeys();  // trigger
+    forall key:Key | AnyKey(key)
+      ensures I(v').stampedBetree.root.children.mapp[key]
+          == PagedBetree.ConstantChildMap(I(v).stampedBetree.root).mapp[key] {
+      AllKeysInTotalDomain(key);
+    }
+  }
+
+  lemma SubstitutionEquivalenceRefines(path: Path, target': BetreeNode)
+    requires path.Valid()
+    requires INode(target') == INode(path.Target())
+    ensures INode(path.node) == INode(path.Substitute(target'))
+  {
+    assume false;
+  }
+
+  lemma SplitEquivalence(step: Step)
+    requires step.InternalSplitStep?
+    requires step.path.Valid()
+    requires step.path.Target().CanSplit(step.childIdx, step.splitKey)
+    ensures INode(step.path.node.Split(step.childIdx, step.splitKey))
+      == INode(step.path.node).Split(SplitLeftKeys(step), SplitChildKeys(step) - SplitLeftKeys(step));
+  {
+  }
+
+  lemma {:timeLimitMultiplier 2} InternalSplitStepRefines(v: Variables, v': Variables, lbl: TransitionLabel, step: Step)
+    requires Inv(v)
+    requires NextStep(v, v', lbl, step)
+    requires step.InternalSplitStep?
+    ensures v'.WF()
+    ensures PagedBetree.NextStep(I(v), I(v'), ILbl(lbl), IStep(v, v', lbl, step))
+  {
+    INodeWF(v.stampedBetree.root);
+    INodeWF(step.path.Target());
+    InvNext(v, v', lbl);
+    assert v'.WF();
+    INodeWF(v'.stampedBetree.root);
+    assert step.path.Valid();
+    ValidPathRefines(step.path);
+    assert IPath(step.path).Valid();
+    var target' := step.path.Target().Split(step.childIdx, step.splitKey);
+    //SplitEquivalence(step.path.Target(), step.childIdx, step.splitKey);
+    SplitEquivalence(step);
+    SubstitutionEquivalenceRefines(step.path, target');
+    var istep := IStep(v, v', lbl, step);
+    var itarget' := istep.path.Target().Split(istep.leftKeys, istep.rightKeys);
+    var iv := I(v);
+    var iv' := I(v');
+
+    PathTargetRefines(step.path);
+    calc {
+      itarget';
+      istep.path.Target().Split(istep.leftKeys, istep.rightKeys);
+      INode(target');
+    }
+
+    assert iv.stampedBetree.root == INode(v.stampedBetree.root);
+    assert iv.stampedBetree.root == istep.path.node;
+    assert istep.path.Target() == INode(step.path.Target());
+    assert iv'.stampedBetree.root == INode(v'.stampedBetree.root);
+    assert itarget' == INode(target');
+
+    assert iv'.stampedBetree.root == istep.path.Substitute(istep.path.Target().Split(istep.leftKeys, istep.rightKeys));
+    assert PagedBetree.InternalSplit(I(v), I(v'), ILbl(lbl), IStep(v, v', lbl, step));
+  }
+
+  lemma NextRefines(v: Variables, v': Variables, lbl: TransitionLabel)
+    requires Inv(v)
+    requires Next(v, v', lbl)
+    ensures v'.WF()
+    ensures PagedBetree.Next(I(v), I(v'), ILbl(lbl))
+  {
+    InvNext(v, v', lbl);
+    var step: Step :| NextStep(v, v', lbl, step);
+    match step {
+      case QueryStep(receipt) => {
+        ValidReceiptRefines(step.receipt);
+        assert PagedBetree.NextStep(I(v), I(v'), ILbl(lbl), IStep(v, v', lbl, step)); // trigger
+      }
+      case PutStep() => {
+        assert PagedBetree.NextStep(I(v), I(v'), ILbl(lbl), IStep(v, v', lbl, step));
+      }
+      case QueryEndLsnStep() => {
+        assert PagedBetree.NextStep(I(v), I(v'), ILbl(lbl), IStep(v, v', lbl, step));
+      }
+      case FreezeAsStep() => {
+        INodeWF(v.stampedBetree.root);
+        assert PagedBetree.NextStep(I(v), I(v'), ILbl(lbl), IStep(v, v', lbl, step)); // trigger
+      }
+      case InternalGrowStep() => {
+        InternalGrowStepRefines(v, v', lbl, step);
+      }
+      case InternalSplitStep(_, _, _) => {
+        assume PagedBetree.NextStep(I(v), I(v'), ILbl(lbl), IStep(v, v', lbl, step));
+      }
+      case InternalFlushStep(_, _) => {
+        assume PagedBetree.NextStep(I(v), I(v'), ILbl(lbl), IStep(v, v', lbl, step));
+      }
+      case InternalCompactStep(_, _) => {
+        assume PagedBetree.NextStep(I(v), I(v'), ILbl(lbl), IStep(v, v', lbl, step));
+      }
+    }
+  }
 }
