Splinter/BlockLayer/BlockCoordinationSystem.i.dfy
@@ -62,12 +62,17 @@ module BlockCoordinationSystem {
     }
   }
 
+  function SimpleLabel(clbl: CrashTolerantJournal.TransitionLabel) : BlockCrashTolerantJournal.TransitionLabel
+  {
+    TransitionLabel({}, CrashTolerantJournal.LoadEphemeralFromPersistentLabel())
+  }
+
   predicate LoadEphemeralFromPersistent(v: Variables, v': Variables, uiop : UIOp)
   {
     && v.WF()
     && uiop.NoopOp?
     && v'.ephemeral.Known?
-    && BlockCrashTolerantJournal.Next(v.journal, v'.journal, CrashTolerantJournal.LoadEphemeralFromPersistentLabel())
+    && BlockCrashTolerantJournal.Next(v.journal, v'.journal, SimpleLabel(CrashTolerantJournal.LoadEphemeralFromPersistentLabel()))
     && BlockCrashTolerantMap.Next(v.mapadt, v'.mapadt, CrashTolerantMap.LoadEphemeralFromPersistentLabel(v'.ephemeral.mapLsn))
     && v'.ephemeral.progress == Async.InitEphemeralState()
     && v'.ephemeral.syncReqs == map[]
@@ -87,7 +92,7 @@ module BlockCoordinationSystem {
 
     // NB that Recover can interleave with mapadt steps (the Betree
     // reorganizing its state, possibly flushing stuff out to disk).
-    && BlockCrashTolerantJournal.Next(v.journal, v'.journal, CrashTolerantJournal.ReadForRecoveryLabel(records))
+    && BlockCrashTolerantJournal.Next(v.journal, v'.journal, SimpleLabel(CrashTolerantJournal.ReadForRecoveryLabel(records)))
     && BlockCrashTolerantMap.Next(v.mapadt, v'.mapadt, CrashTolerantMap.PutRecordsLabel(records))
 
     && v'.ephemeral == v.ephemeral.(mapLsn := records.seqEnd) // all else defined via predicates above
@@ -123,7 +128,7 @@ module BlockCoordinationSystem {
     && assert AnyKey(key);
 
     // Journal confirms that the map is up-to-date (but otherwise doesn't do anything).
-    && BlockCrashTolerantJournal.Next(v.journal, v'.journal, CrashTolerantJournal.QueryEndLsnLabel(v.ephemeral.mapLsn))
+    && BlockCrashTolerantJournal.Next(v.journal, v'.journal, SimpleLabel(CrashTolerantJournal.QueryEndLsnLabel(v.ephemeral.mapLsn)))
     // Map handles the query
     && BlockCrashTolerantMap.Next(v.mapadt, v'.mapadt, CrashTolerantMap.QueryLabel(v.ephemeral.mapLsn, key, value))
 
@@ -159,7 +164,7 @@ module BlockCoordinationSystem {
     && var singleton := MsgHistoryMod.SingletonAt(v.ephemeral.mapLsn, KeyedMessage(key, Define(val)));
 
     && v.WF()
-    && BlockCrashTolerantJournal.Next(v.journal, v'.journal, CrashTolerantJournal.PutLabel(singleton))
+    && BlockCrashTolerantJournal.Next(v.journal, v'.journal, SimpleLabel(CrashTolerantJournal.PutLabel(singleton)))
     && BlockCrashTolerantMap.Next(v.mapadt, v'.mapadt, CrashTolerantMap.PutRecordsLabel(singleton))
 
     && v'.ephemeral == v.ephemeral.(
@@ -192,7 +197,7 @@ module BlockCoordinationSystem {
     && v.ephemeral.Known?
     && v'.ephemeral.Known?
     && uiop.NoopOp?
-    && BlockCrashTolerantJournal.Next(v.journal, v'.journal, CrashTolerantJournal.InternalLabel())
+    && BlockCrashTolerantJournal.Next(v.journal, v'.journal, SimpleLabel(CrashTolerantJournal.InternalLabel()))
     && v' == v.(journal := v'.journal)  // predicate update above
   }
 
@@ -218,7 +223,7 @@ module BlockCoordinationSystem {
     // Need to record the current LSN, which is generally the current map state. But we
     // also need to confirm that the journal hasn't gone ahead, since sync is relative to
     // writes (which have affected the journal).
-    && BlockCrashTolerantJournal.Next(v.journal, v'.journal, CrashTolerantJournal.QueryEndLsnLabel(v.ephemeral.mapLsn))
+    && BlockCrashTolerantJournal.Next(v.journal, v'.journal, SimpleLabel(CrashTolerantJournal.QueryEndLsnLabel(v.ephemeral.mapLsn)))
 
     && v'.mapadt == v.mapadt
 
@@ -234,7 +239,7 @@ module BlockCoordinationSystem {
     && v.ephemeral.Known?
     && uiop.ReplySyncOp?
     && uiop.syncReqId in v.ephemeral.syncReqs
-    && BlockCrashTolerantJournal.Next(v.journal, v'.journal, CrashTolerantJournal.QueryLsnPersistenceLabel(v.ephemeral.syncReqs[uiop.syncReqId]))
+    && BlockCrashTolerantJournal.Next(v.journal, v'.journal, SimpleLabel(CrashTolerantJournal.QueryLsnPersistenceLabel(v.ephemeral.syncReqs[uiop.syncReqId])))
     && v' == v.(ephemeral := v.ephemeral.(
         syncReqs := MapRemove1(v.ephemeral.syncReqs, uiop.syncReqId)
       ))
@@ -247,7 +252,7 @@ module BlockCoordinationSystem {
     && v.WF()
     && v.ephemeral.Known?
 
-    && BlockCrashTolerantJournal.Next(v.journal, v'.journal, CrashTolerantJournal.CommitStartLabel(newBoundaryLsn, v.ephemeral.mapLsn))
+    && BlockCrashTolerantJournal.Next(v.journal, v'.journal, SimpleLabel(CrashTolerantJournal.CommitStartLabel(newBoundaryLsn, v.ephemeral.mapLsn)))
     && BlockCrashTolerantMap.Next(v.mapadt, v'.mapadt, CrashTolerantMap.CommitStartLabel(newBoundaryLsn))
 
     && v'.ephemeral == v.ephemeral  // UNCHANGED
@@ -261,7 +266,7 @@ module BlockCoordinationSystem {
     && uiop.SyncOp?
     && v.ephemeral.Known? // provable from invariant
 
-    && BlockCrashTolerantJournal.Next(v.journal, v'.journal, CrashTolerantJournal.CommitCompleteLabel(v.ephemeral.mapLsn))
+    && BlockCrashTolerantJournal.Next(v.journal, v'.journal, SimpleLabel(CrashTolerantJournal.CommitCompleteLabel(v.ephemeral.mapLsn)))
     && BlockCrashTolerantMap.Next(v.mapadt, v'.mapadt, CrashTolerantMap.CommitCompleteLabel())
 
     && v'.ephemeral == v.ephemeral  // UNCHANGED
@@ -273,7 +278,7 @@ module BlockCoordinationSystem {
     && v'.WF()
     && uiop.CrashOp?
 
-    && BlockCrashTolerantJournal.Next(v.journal, v'.journal, CrashTolerantJournal.CrashLabel())
+    && BlockCrashTolerantJournal.Next(v.journal, v'.journal, SimpleLabel(CrashTolerantJournal.CrashLabel()))
     && BlockCrashTolerantMap.Next(v.mapadt, v'.mapadt, CrashTolerantMap.CrashLabel())
 
     && v'.ephemeral.Unknown?
